WIP: Half the proof of incrementality of SHA3

specs/lemmas/Spec.SHA3.Incremental.fst
@@ -16,111 +16,158 @@ module UpdateMulti = Lib.UpdateMulti
 
 open Lib.IntTypes
 
-#set-options "--fuel 0 --ifuel 0 --z3rlimit 50"
+#set-options "--fuel 0 --ifuel 0 --z3rlimit 200"
 
-(*
+let update_is_update_multi (a:sha3_alg) (inp:bytes{S.length inp == block_length a}) (s:words_state a)
+  : Lemma (Spec.SHA3.absorb_inner (1088/8) inp s == update_multi a s () inp)
+  = let rateInBytes = 1088/8 in
+    let f = Spec.SHA3.absorb_inner rateInBytes in
+    let bs = block_length a in
+    let f' = Lib.Sequence.repeat_blocks_f bs inp f 1 in
+    assert (bs == rateInBytes);
+    calc (==) {
+      update_multi a s () inp;
+      (==) { }
+      Lib.Sequence.repeat_blocks_multi #_ #(words_state a) rateInBytes inp f s;
+      (==) { Lib.Sequence.lemma_repeat_blocks_multi #_ #(words_state a) bs inp f s }
+      (let len = S.length inp in
+       let nb = len / bs in
+      Loops.repeati #(words_state a) nb (Lib.Sequence.repeat_blocks_f bs inp f nb) s);
+      (==) {
+        Loops.unfold_repeati 1 f' s 0;
+        Loops.eq_repeati0 1 f' s }
+      f' 0 s;
+      (==) { assert (Seq.slice inp (0 * bs) (0 * bs + bs) `S.equal` inp) }
+      f inp s;
+    }
+
 let sha3_is_incremental1
   (a: sha3_alg)
   (input: bytes): Lemma (hash_incremental a input `S.equal` (
     let s = Lib.Sequence.create 25 (u64 0) in
-    let s = coerce #(words_state a) #(Lib.Sequence.lseq uint64 25) s in
     let rateInBytes = 1088 / 8 in
     let delimitedSuffix = byte 0x06 in
     let bs, l = UpdateMulti.split_at_last rateInBytes input in
-    let s = update_multi a s bs in
+    let s = update_multi a s () bs in
     let s = Spec.SHA3.absorb_last delimitedSuffix rateInBytes (S.length l) l s in
     finish a s))
-=
+= calc (==) {
+       hash_incremental a input;
+       (==) { }
+       (let s = init a in
+        let bs, l = split_blocks a input in
+        let s = update_multi a s () bs in
+        let s = update_last a s (S.length bs) l in
+        finish a s);
+       (==) { }
+       (let s = Lib.Sequence.create 25 (u64 0) in
+        let rateInBytes = 1088/8 in
+        let bs, l = UpdateMulti.split_at_last_lazy rateInBytes input in
+        let s = update_multi a s () bs in
+        let s = update_last a s (S.length bs) l in
+        finish a s);
+       (==) { } (
+       let s = Lib.Sequence.create 25 (u64 0) in
+       let rateInBytes = 1088 / 8 in
+       let delimitedSuffix = byte 0x06 in
+       let bs, l = UpdateMulti.split_at_last_lazy rateInBytes input in
+       if S.length l = rateInBytes then
+         let s = update_multi a s () bs in
+         let s = Spec.SHA3.absorb_inner rateInBytes l s in
+         let s = Spec.SHA3.absorb_last delimitedSuffix rateInBytes 0 S.empty s in
+         finish a s
+       else
+         let s = update_multi a s () bs in
+         let s = Spec.SHA3.absorb_last delimitedSuffix rateInBytes (S.length l) l s in
+       finish a s
+       );
+       (==) { (
+         let s = Lib.Sequence.create 25 (u64 0) in
+         let rateInBytes = 1088 / 8 in
+         let delimitedSuffix = byte 0x06 in
+         let bs, l = UpdateMulti.split_at_last_lazy rateInBytes input in
+         if S.length l = rateInBytes then
+           let s = update_multi a s () bs in
+           update_is_update_multi a l s
+         else ()
+         ) } (
+       let s = Lib.Sequence.create 25 (u64 0) in
+       let rateInBytes = 1088 / 8 in
+       let delimitedSuffix = byte 0x06 in
+       let bs, l = UpdateMulti.split_at_last_lazy rateInBytes input in
+       if S.length l = rateInBytes then
+         let s = update_multi a s () bs in
+         let s = update_multi a s () l in
+         let s = Spec.SHA3.absorb_last delimitedSuffix rateInBytes 0 S.empty s in
+         finish a s
+       else
+         let s = update_multi a s () bs in
+         let s = Spec.SHA3.absorb_last delimitedSuffix rateInBytes (S.length l) l s in
+       finish a s
+       );
+       (==) { (
+         let s = Lib.Sequence.create 25 (u64 0) in
+         let rateInBytes = 1088 / 8 in
+         let delimitedSuffix = byte 0x06 in
+         let bs, l = UpdateMulti.split_at_last_lazy rateInBytes input in
+         if S.length l = rateInBytes then
+           Lib.Sequence.Lemmas.repeat_blocks_multi_split (block_length a) (S.length bs) (bs `S.append` l) (Spec.SHA3.absorb_inner rateInBytes) s
+         else () ) } (
+       let s = Lib.Sequence.create 25 (u64 0) in
+       let rateInBytes = 1088 / 8 in
+       let delimitedSuffix = byte 0x06 in
+       let bs, l = UpdateMulti.split_at_last_lazy rateInBytes input in
+       if S.length l = rateInBytes then
+         let s = update_multi a s () (bs `S.append` l) in
+         let s = Spec.SHA3.absorb_last delimitedSuffix rateInBytes 0 S.empty s in
+         finish a s
+       else
+         let s = update_multi a s () bs in
+         let s = Spec.SHA3.absorb_last delimitedSuffix rateInBytes (S.length l) l s in
+       finish a s
+       );
+  };
   calc (S.equal) {
-    hash_incremental a input;
-  (S.equal) { } (
-    let s = Lib.Sequence.create 25 (u64 0) in
-    let s = coerce #(words_state a) #(Lib.Sequence.lseq uint64 25) s in
-    let bs, l = split_blocks a input in
-    let s = update_multi a s bs in
-    let s = update_last a s (S.length bs) l in
-    finish a s
-  );
-  (S.equal) { } (
-    let s = Lib.Sequence.create 25 (u64 0) in
-    let s = coerce #(words_state a) #(Lib.Sequence.lseq uint64 25) s in
-    // Also the block size
-    let rateInBytes = 1088 / 8 in
-    let delimitedSuffix = byte 0x06 in
-    let bs, l = UpdateMulti.split_at_last_lazy rateInBytes input in
-    let s = update_multi a s bs in
-    let s = update_last a s (S.length bs) l in
-    finish a s
-  );
-  (S.equal) { } (
-    let s = Lib.Sequence.create 25 (u64 0) in
-    let s = coerce #(words_state a) #(Lib.Sequence.lseq uint64 25) s in
-    // Also the block size
-    let rateInBytes = 1088 / 8 in
-    let delimitedSuffix = byte 0x06 in
-    let bs, l = UpdateMulti.split_at_last_lazy rateInBytes input in
-    let s = update_multi a s bs in
-    if S.length l = rateInBytes then
-      let s = update SHA3_256 s l in
-      let s = Spec.SHA3.absorb_last delimitedSuffix rateInBytes 0 S.empty s in
-      finish a s
-    else
-      let s = s in
-      let s = Spec.SHA3.absorb_last delimitedSuffix rateInBytes (S.length l) l s in
-      finish a s
-  );
-  (S.equal) {
-    let s = Lib.Sequence.create 25 (u64 0) in
-    let s = coerce #(words_state a) #(Lib.Sequence.lseq uint64 25) s in
-    let rateInBytes = 1088 / 8 in
-    let bs, l = UpdateMulti.split_at_last_lazy rateInBytes input in
-    let s = update_multi a s bs in
-    if S.length l = rateInBytes then
-      Lib.UpdateMulti.update_multi_associative rateInBytes (update a) s bs l
-    else
-      ()
-  } (
-    let s = Lib.Sequence.create 25 (u64 0) in
-    let s = coerce #(words_state a) #(Lib.Sequence.lseq uint64 25) s in
-    // Also the block size
-    let rateInBytes = 1088 / 8 in
-    let delimitedSuffix = byte 0x06 in
-    let bs, l = UpdateMulti.split_at_last rateInBytes input in
-    if S.length l = rateInBytes then
-      let s = update_multi a s (bs `S.append` l) in
-      let s = Spec.SHA3.absorb_last delimitedSuffix rateInBytes 0 S.empty s in
-      finish a s
-    else
-      let s= update_multi a s bs in
-      let s = Spec.SHA3.absorb_last delimitedSuffix rateInBytes (S.length l) l s in
-      finish a s
-  );
-  (S.equal) {
-    let s = Lib.Sequence.create 25 (u64 0) in
-    let s = coerce #(words_state a) #(Lib.Sequence.lseq uint64 25) s in
-    let rateInBytes = 1088 / 8 in
-    let bs, l = UpdateMulti.split_at_last_lazy rateInBytes input in
-    let s = update_multi a s bs in
-    if S.length l = rateInBytes then begin
-      let bs', l' = UpdateMulti.split_at_last rateInBytes input in
-      // TODO: strengthen this... NL arith!
-      assert (bs' `S.equal` (bs `S.append` l));
-      assert (l' `S.equal` S.empty)
-    end else
-      ()
-  } (
-    let s = Lib.Sequence.create 25 (u64 0) in
-    let s = coerce #(words_state a) #(Lib.Sequence.lseq uint64 25) s in
-    // Also the block size
-    let rateInBytes = 1088 / 8 in
-    let delimitedSuffix = byte 0x06 in
-    let bs, l = UpdateMulti.split_at_last rateInBytes input in
-    let s = update_multi a s bs in
-    let s = Spec.SHA3.absorb_last delimitedSuffix rateInBytes (S.length l) l s in
-    finish a s
-  );
+    (
+       let s = Lib.Sequence.create 25 (u64 0) in
+       let rateInBytes = 1088 / 8 in
+       let delimitedSuffix = byte 0x06 in
+       let bs, l = UpdateMulti.split_at_last_lazy rateInBytes input in
+       if S.length l = rateInBytes then
+         let s = update_multi a s () (bs `S.append` l) in
+         let s = Spec.SHA3.absorb_last delimitedSuffix rateInBytes 0 S.empty s in
+         finish a s
+       else
+         let s = update_multi a s () bs in
+         let s = Spec.SHA3.absorb_last delimitedSuffix rateInBytes (S.length l) l s in
+       finish a s
+       );
+
+       (S.equal) {
+       let s = Lib.Sequence.create 25 (u64 0) in
+       let rateInBytes = 1088 / 8 in
+       let bs, l = UpdateMulti.split_at_last_lazy rateInBytes input in
+       let s = update_multi a s () bs in
+       if S.length l = rateInBytes then begin
+         let bs', l' = UpdateMulti.split_at_last rateInBytes input in
+         // TODO: strengthen this... NL arith!
+         assert (bs' `S.equal` (bs `S.append` l));
+         assert (l' `S.equal` S.empty)
+       end else
+         ()
+     } (
+       let s = Lib.Sequence.create 25 (u64 0) in
+       // Also the block size
+       let rateInBytes = 1088 / 8 in
+       let delimitedSuffix = byte 0x06 in
+       let bs, l = UpdateMulti.split_at_last rateInBytes input in
+       let s = update_multi a s () bs in
+       let s = Spec.SHA3.absorb_last delimitedSuffix rateInBytes (S.length l) l s in
+       finish a s
+     );
   }
 
+(*
 let sha3_update (a: sha3_alg) (s: words_state' a) (b: bytes { S.length b = block_length a }): words_state' a =
     let rateInBytes = 1088 / 8 in
   Spec.SHA3.absorb_inner rateInBytes b s
@@ -148,18 +195,21 @@ let rec sha3_ignores_extra_state (a: sha3_alg) (acc: words_state' a) (bs: bytes)
     let acc = sha3_update a acc block in
     sha3_ignores_extra_state a acc rem
 #pop-options
+*)
 
 let sha3_is_incremental2
   (a: sha3_alg)
   (input: bytes): Lemma (hash a input `S.equal` (
-    let s = Lib.Sequence.create 25 (u64 0), () in
+    let s = Lib.Sequence.create 25 (u64 0) in
     let rateInBytes = 1088 / 8 in
     let delimitedSuffix = byte 0x06 in
     let bs, l = UpdateMulti.split_at_last rateInBytes input in
-    let s, _ = update_multi a s bs in
-    let s = Spec.SHA3.absorb_last delimitedSuffix rateInBytes (S.length l) l s, () in
+    let s = update_multi a s () bs in
+    let s = Spec.SHA3.absorb_last delimitedSuffix rateInBytes (S.length l) l s in
     finish a s))
-=
+= admit()
+
+(*
   calc (S.equal) { (
     let s = Lib.Sequence.create 25 (u64 0), () in
     let rateInBytes = 1088 / 8 in
@@ -272,21 +322,21 @@ let sha3_is_incremental2
     Spec.SHA3.sha3_256 (S.length input) input;
   }
 *)
-
 let sha3_is_incremental
   (a: sha3_alg)
   (input: bytes): Lemma (hash_incremental a input `S.equal` hash a input)
-= admit ()
-  // calc (S.equal) {
-  //   hash_incremental a input;
-  // (S.equal) { sha3_is_incremental1 a input } (
-  //   let s = Lib.Sequence.create 25 (u64 0), () in
-  //   let rateInBytes = 1088 / 8 in
-  //   let delimitedSuffix = byte 0x06 in
-  //   let bs, l = UpdateMulti.split_at_last rateInBytes input in
-  //   let s, _ = update_multi a s bs in
-  //   let s = Spec.SHA3.absorb_last delimitedSuffix rateInBytes (S.length l) l s, () in
-  //   finish a s);
-  // (S.equal) { sha3_is_incremental2 a input }
-  //   hash a input;
-  // }
+=
+  assert (hash a input == Spec.SHA3.keccak 1088 512 (S.length input) input (byte 0x06) 32);
+  calc (S.equal) {
+    hash_incremental a input;
+  (S.equal) { sha3_is_incremental1 a input } (
+    let s = Lib.Sequence.create 25 (u64 0) in
+    let rateInBytes = 1088 / 8 in
+    let delimitedSuffix = byte 0x06 in
+    let bs, l = UpdateMulti.split_at_last rateInBytes input in
+    let s = update_multi a s () bs in
+    let s = Spec.SHA3.absorb_last delimitedSuffix rateInBytes (S.length l) l s in
+    finish a s);
+  (S.equal) { sha3_is_incremental2 a input }
+    hash a input;
+  }
